Start semantics of Core Cmm

cmmCore/CmmCoreType.v
@@ -2,6 +2,7 @@
 Require Import Eqdep.
 
 Require Import compcert.lib.Integers.
+Require Import compcert.lib.Floats.
 
 Require Import GHC.CmmType.
 Require Import GHC.Int.
@@ -47,3 +48,44 @@ Definition CC_cmmFloat (w : {w' : Width | isFloatWidth w'}) : CC_CmmType :=
 
 Definition b64 : CC_CmmType := CC_cmmBits (exist _ W64 I).
 Definition bWord : CC_CmmType := CC_cmmBits (exist _ W64 I). (* Need DynFlags here *) 
+
+(* Semantics *)
+
+Module Wordsize_16.
+  Definition wordsize := 16%nat.
+  Remark wordsize_not_zero: wordsize <> 0%nat.
+  Proof. unfold wordsize; congruence. Qed.
+End Wordsize_16.
+
+Strategy opaque [Wordsize_16.wordsize].
+
+Module Int16 := Make(Wordsize_16).
+
+Strategy 0 [Wordsize_16.wordsize].
+
+Notation short := Int16.int.
+
+Notation long := Int64.int.
+
+Definition CC_CmmTypeDenote (ct:CC_CmmType): Type :=
+  match ct with
+  | exist t pf => match t with
+                  | CT_CmmType BitsCat w => match w with
+                                            | W8 => byte
+                                            | W16 => short
+                                            | W32 => int
+                                            | W64 => long
+                                            | _ => unit
+                                            end
+                  | CT_CmmType FloatCat w => match w with
+                                             | W32 => float32
+                                             | W64 => float
+                                             | _ => unit
+                                             end
+                  | CT_CmmType GcPtrCat _ => long
+                  | CT_CmmType (VecCat _ _) _ => unit
+                  end
+  end.
+
+(* We want to make use of CC_CmmType proof here so we don't have to return
+a bogus unit type *)
